1. Prove lemma data_at__tarray_value_join to join two data_at_ together 2. Define relations to represent relations between graphs before and after exection of resume.

CertiGC/spatial_gcgraph.v
@@ -26,35 +26,36 @@ Definition fun_info_rep (sh: share) (fi: fun_info) (p: val) : mpred :=
     sh (tarray tuint (len + 2))
     (map Vint (map Int.repr (fun_word_size fi :: len :: live_roots_indices fi))) p.
 
-Definition space_rest_rep (sp: space): mpred :=
+Definition space_rest_rep (sh: share) (sp: space): mpred :=
   if (Val.eq sp.(space_start) nullval)
   then emp
-  else data_at_ Tsh (tarray int_or_ptr_type (sp.(total_space) - sp.(used_space)))
-                (offset_val sp.(used_space) sp.(space_start)).
+  else data_at_ sh (tarray int_or_ptr_type (sp.(total_space) - sp.(used_space)))
+                (offset_val (WORD_SIZE * used_space sp) sp.(space_start)).
 
-Definition heap_rest_rep (hp: heap): mpred := iter_sepcon hp.(spaces) space_rest_rep.
+Definition heap_rest_rep (sh: share) (hp: heap): mpred :=
+  iter_sepcon hp.(spaces) (space_rest_rep sh).
 
 Definition space_rep (sp: space): (reptype space_type) :=
   let s := sp.(space_start) in (s, (offset_val (WORD_SIZE * sp.(used_space)) s,
                                     offset_val (WORD_SIZE * sp.(total_space)) s)).
 
-Definition heap_struct_rep (sp_reps: list (reptype space_type)) (h: val): mpred :=
-  data_at Tsh heap_type sp_reps h.
+Definition heap_struct_rep (sh: share) (sp_reps: list (reptype space_type)) (h: val):
+  mpred := data_at sh heap_type sp_reps h.
 
-Definition thread_info_rep (ti: thread_info) (t: val) :=
+Definition thread_info_rep (sh: share) (ti: thread_info) (t: val) :=
   if Val.eq ti.(ti_heap_p) nullval
-  then data_at Tsh thread_info_type
+  then data_at sh thread_info_type
                (Vundef, (Vundef, (nullval, list_repeat (Z.to_nat MAX_ARGS) Vundef))) t
   else let nursery := heap_head ti.(ti_heap) in
        let p := nursery.(space_start) in
        let n_lim := offset_val (WORD_SIZE * nursery.(total_space)) p in
-       data_at Tsh thread_info_type
+       data_at sh thread_info_type
                (offset_val (WORD_SIZE * nursery.(used_space)) p,
                 (n_lim, (ti.(ti_heap_p), ti.(ti_args)))) t *
        heap_struct_rep
-         ((p, (Vundef, n_lim))
-            :: map space_rep (tl ti.(ti_heap).(spaces))) ti.(ti_heap_p) *
-       heap_rest_rep ti.(ti_heap).
+         sh ((p, (Vundef, n_lim))
+               :: map space_rep (tl ti.(ti_heap).(spaces))) ti.(ti_heap_p) *
+       heap_rest_rep sh ti.(ti_heap).
 
 Definition outlier_rep (outlier: outlier_t) :=
   fold_right andp TT (map (compose valid_pointer GC_Pointer2val) outlier).
@@ -203,4 +204,57 @@ Proof.
   sep_apply (generation_rep_memory_block sh g gen num).
   rewrite <- sizeof_tarray_int_or_ptr by apply previous_size_ge_zero.
   rewrite memory_block_data_at_; auto.
+Qed.
+
+Lemma data_at__tarray_value_join_local_fact: forall sh n n1 p,
+    0 <= n1 <= n ->
+    data_at_ sh (tarray int_or_ptr_type n1) p *
+    data_at_ sh (tarray int_or_ptr_type (n - n1)) (offset_val (WORD_SIZE * n1) p) |--
+             !!(field_compatible (tarray int_or_ptr_type n) [] p).
+Proof.
+  intros. entailer!. unfold field_compatible. simpl. destruct H0 as [? [_ [? [? _]]]].
+  destruct H1 as [_ [_ [? [? _]]]]. destruct p; try contradiction. clear H0.
+  simpl isptr. inv_int i. unfold size_compatible in *. simpl in H1.
+  rewrite sizeof_tarray_int_or_ptr in * by omega. rewrite WORD_SIZE_eq in *.
+  rewrite ptrofs_add_repr in H1. do 2 rewrite Ptrofs.unsigned_repr in * by rep_omega.
+  replace (Z.max 0 (n - n1)) with (n - n1) in H1 by (rewrite Z.max_r; omega).
+  assert (ofs + 4 * n < Ptrofs.modulus) by omega. intuition. constructor. intros.
+  simpl sizeof. rewrite Ptrofs.unsigned_repr by rep_omega.
+  apply align_compatible_rec_by_value with Mptr. 1: reflexivity. simpl.
+  apply Z.divide_add_r. 2: apply Z.divide_factor_l. simpl offset_val in H4.
+  rewrite ptrofs_add_repr in H4. unfold align_compatible in *.
+  rewrite Ptrofs.unsigned_repr in * by rep_omega.
+  pose proof (align_compatible_rec_Tarray_inv _ _ _ _ _ H3).
+  pose proof (align_compatible_rec_Tarray_inv _ _ _ _ _ H4). simpl sizeof in *.
+  rewrite Z.le_lteq in H6. destruct H6.
+  - assert (0 <= 0 < n1) by omega. specialize (H9 _ H11).
+    apply (align_compatible_rec_by_value_inv _ _ Mptr) in H9. 2: reflexivity.
+    simpl in H9. rewrite Z.add_0_r in H9. assumption.
+  - subst n1. rewrite Z.sub_0_r in H10. specialize (H10 _ H5).
+    apply (align_compatible_rec_by_value_inv _ _ Mptr) in H10. 2: reflexivity.
+    simpl in H10. rewrite Z.add_0_r, Z.add_comm in H10.
+    apply Z.divide_add_cancel_r in H10; [assumption | apply Z.divide_factor_l].
+Qed.
+
+Lemma data_at__tarray_value_join: forall sh n n1 p,
+    0 <= n1 <= n -> 
+    data_at_ sh (tarray int_or_ptr_type n1) p *
+    data_at_ sh (tarray int_or_ptr_type (n - n1)) (offset_val (WORD_SIZE * n1) p) |--
+             data_at_ sh (tarray int_or_ptr_type n) p.
+Proof.
+  intros. unfold data_at_ at 3; unfold field_at_. rewrite field_at_data_at.
+  erewrite (@split2_data_at_Tarray CompSpecs sh int_or_ptr_type n n1).
+  - instantiate (1:= list_repeat (Z.to_nat (n-n1)) Vundef).
+    instantiate (1:= list_repeat (Z.to_nat n1) Vundef). unfold field_address. simpl.
+    sep_apply (data_at__tarray_value_join_local_fact sh n n1 p H). Intros.
+    rewrite if_true; trivial. entailer!. unfold data_at_. unfold field_at_.
+    rewrite field_at_data_at. unfold field_address0. rewrite if_true.
+    + simpl. unfold field_address. rewrite if_true; trivial. simpl.
+      rewrite offset_offset_val. entailer!.
+    + unfold field_compatible0. simpl. destruct H0. intuition.
+  - assumption.
+  - instantiate (1:=list_repeat (Z.to_nat n) Vundef). list_solve.
+  - unfold default_val. simpl. autorewrite with sublist. apply JMeq_refl. 
+  - unfold default_val. simpl. autorewrite with sublist. apply JMeq_refl. 
+  - unfold default_val. simpl. autorewrite with sublist. apply JMeq_refl.
 Qed.
